examples/Drinks_Machine.thy
@@ -83,7 +83,7 @@ lemma possible_steps_0:
   by (simp_all add: transitions apply_guards_def)
 
 lemma first_step_select:
-  "(s', T) |\<in>| possible_steps drinks 0 r aa b \<Longrightarrow> s' = 1 \<and> T = select"
+  "(s', t) |\<in>| possible_steps drinks 0 r aa b \<Longrightarrow> s' = 1 \<and> t = select"
   apply (simp add: possible_steps_def fimage_def ffilter_def fmember_def Abs_fset_inverse Set.filter_def drinks_def)
   apply safe
   by (simp_all add: transitions)
