examples/Drinks_Machine_2.thy
@@ -249,87 +249,64 @@ lemma drinks2_vend_invalid:
   apply safe
   by (simp_all add: transitions can_take_transition_def can_take_def value_gt_def MaybeBoolInt_not_num_1)
 
-lemma equiv_1_2: "observe_execution drinks 1 r t = observe_execution drinks2 2 r t"
-proof(induct t arbitrary: r)
+lemma equiv_1_2: "executionally_equivalent drinks 1 r drinks2 2 r x"
+proof(induct x arbitrary: r)
   case Nil
   then show ?case
     by simp
 next
   case (Cons a t)
   then show ?case
+    apply (cases a, clarsimp)
+    apply (rule executionally_equivalent.step)
     apply (case_tac "fst a = STR ''coin'' \<and> length (snd a) = 1")
-     defer
-     apply (case_tac "a = (STR ''vend'', [])")
-      defer
-      apply (rule observe_execution_no_possible_steps)
-       apply (simp add: drinks_1_rejects)
-      apply (simp add: drinks2_2_invalid)
-     apply (rule observe_execution_one_possible_step)
-          apply (simp add: possible_steps_1_coin)
-         apply (simp add: possible_steps_2_coin)
-        apply simp+
+     defer apply (case_tac "a = (STR ''vend'', [])")
+      defer using drinks2_2_invalid drinks_no_possible_steps_1 apply auto[1]
+    apply (simp add: Drinks_Machine.possible_steps_1_coin possible_steps_2_coin)
     apply (case_tac "\<exists>n. r $ 2 = Some (Num n)")
-     defer
-     apply (simp add: drinks_vend_invalid drinks2_vend_invalid)
+     defer using drinks_vend_invalid drinks2_vend_invalid apply simp
     apply clarify
     apply (case_tac "n < 100")
      apply (simp add: Drinks_Machine.drinks_vend_insufficient drinks2_vend_insufficient2)
     apply (simp add: Drinks_Machine.drinks_vend_sufficient drinks2_vend_sufficient)
     apply (induct t)
      apply simp
-    apply (rule observe_execution_no_possible_steps)
-     apply (simp add: drinks_end)
-    by (simp add: drinks2_end)
+    apply (case_tac aa, clarsimp)
+    by (simp add: executionally_equivalent_step drinks_end drinks2_end)
 qed
 
-lemma equiv_1_1:
-  "observe_execution drinks 1 <2 $:= Some (Num 0), 1 $:= i> t = observe_execution drinks2 1 <2 $:= Some (Num 0), 1 $:= i> t"
-proof(induct t)
+lemma equiv_1_1: "r$2 = Some (Num 0) \<Longrightarrow> executionally_equivalent drinks 1 r drinks2 1 r x"
+proof(induct x)
   case Nil
   then show ?case
     by simp
 next
   case (Cons a t)
   then show ?case
-    apply (case_tac "fst a = STR ''coin'' \<and> length (snd a) = 1")
-     defer
-     apply (case_tac "a = (STR ''vend'', [])")
-      defer
-      apply (rule observe_execution_no_possible_steps)
-       apply (simp add: drinks_1_rejects)
-      apply (metis drinks2_1_invalid prod.collapse)
-     apply (rule observe_execution_one_possible_step)
-          apply (simp add: possible_steps_1_coin)
-         apply (simp add: possible_steps_1)
-        apply simp+
-     apply (simp add: equiv_1_2)
-    apply (rule observe_execution_one_possible_step)
-         apply (simp add: drinks_vend_insufficient)
-        apply (simp add: drinks2_vend_insufficient)
-       apply (simp add: vend_fail_def vend_nothing_def)+
-    by (simp add: datastate(1) finfun_update_twist apply_updates_def)
+    apply (cases a, clarsimp)
+    apply (rule executionally_equivalent.step)
+    apply (case_tac "aa = STR ''coin'' \<and> length b = 1")
+     defer apply (case_tac "a = (STR ''vend'', [])")
+      defer apply (simp add: drinks2_1_invalid drinks_no_possible_steps_1)
+     apply (simp add: Drinks_Machine.possible_steps_1_coin possible_steps_1 equiv_1_2)
+    apply clarsimp
+    apply (simp add: drinks_vend_insufficient drinks2_vend_insufficient)
+    apply (simp add: vend_fail_def vend_nothing_def apply_updates_def)
+    by (metis finfun_upd_triv)
 qed
 
 (* Corresponds to Example 3 in Foster et. al. *)
-lemma observational_equivalence: "observably_equivalent drinks drinks2 t"
-proof (induct t)
-  case Nil
-  then show ?case
-    by (simp add: observably_equivalent_def)
-  next
-  case (Cons a t)
-  then show ?case
-    apply (simp add: observably_equivalent_def)
-    apply (case_tac "fst a = STR ''select'' \<and> length (snd a) = 1")
-     apply (rule observe_execution_one_possible_step)
-          apply (simp add: Drinks_Machine.possible_steps_0)
-         apply (simp add: possible_steps_0)
-       apply simp+
-     apply (simp add: select_def join_ir_def input2state_nth apply_updates_def)
-     apply (metis equiv_1_1 empty_None finfun_update_twist numeral_eq_one_iff semiring_norm(85))
-     apply (rule observe_execution_no_possible_steps)
-    using drinks_0_rejects apply blast
-    using drinks2_0_invalid by auto
-qed
+lemma observational_equivalence: "trace_equivalent drinks drinks2"
+  apply (rule executionally_equivalent_trace_equivalent, clarify)
+  subgoal for x
+    apply (induct x)
+     apply simp
+    apply (case_tac a, clarify)
+    apply (rule executionally_equivalent.step)
+    apply (case_tac "aa = STR ''select'' \<and> length ba = 1")
+     defer using drinks2_0_invalid possible_steps_0_invalid apply auto[1]
+    apply (simp add: Drinks_Machine.possible_steps_0 possible_steps_0)
+    by (simp add: apply_updates_def select_def equiv_1_1)
+  done
 
 end
